Parametricity theorems for Simplicity expressions in Coq.

Coq/Simplicity/Alg.v
@@ -2,26 +2,66 @@ Require Import Simplicity.Ty.
 Require Simplicity.Core.
 
 Set Implicit Arguments.
+Local Open Scope ty_scope.
 
 Module Core.
 
 Module Class.
-Record class (term : Ty -> Ty -> Type) := Class {
-  iden : forall {a:Ty}, term a a;
-  comp : forall {a b c:Ty}, term a b -> term b c -> term a c;
-  unit : forall {a:Ty}, term a Unit;
-  injl : forall {a b c:Ty}, term a b -> term a (Sum b c);
-  injr : forall {a b c:Ty}, term a c -> term a (Sum b c);
-  case : forall {a b c d:Ty}, term (Prod a c) d -> term (Prod b c) d -> term (Prod (Sum a b) c) d;
-  pair : forall {a b c:Ty}, term a b -> term a c -> term a (Prod b c);
-  take : forall {a b c:Ty}, term a c -> term (Prod a b) c;
-  drop : forall {a b c: Ty}, term b c -> term (Prod a b) c
+Record class (term : Ty -> Ty -> Type) := Class
+{ iden : forall {A}, term A A
+; comp : forall {A B C}, term A B -> term B C -> term A C
+; unit : forall {A}, term A Unit
+; injl : forall {A B C}, term A B -> term A (B + C)
+; injr : forall {A B C}, term A C -> term A (B + C)
+; case : forall {A B C D}, term (A * C) D -> term (B * C) D -> term ((A + B) * C) D
+; pair : forall {A B C}, term A B -> term A C -> term A (B * C)
+; take : forall {A B C}, term A C -> term (A * B) C
+; drop : forall {A B C}, term B C -> term (A * B) C
 }.
 End Class.
 
-Structure type := Pack { alg :> Ty -> Ty -> Type; class_of :> Class.class alg }.
+Structure type := Pack { carrier :> Ty -> Ty -> Type; class_of :> Class.class carrier }.
 
-Definition TermAlg : type := Pack (Class.Class
+Record ReynoldsRel (term1 term2 : type) :=
+ { rel :> forall {A B}, term1 A B -> term2 A B -> Prop
+ ; _ : forall A, rel (Class.iden term1) (@Class.iden _ term2 A)
+ ; _ : forall A B C s1 s2 t1 t2, rel s1 s2 -> rel t1 t2 -> rel (Class.comp term1 s1 t1) (@Class.comp _ term2 A B C s2 t2)
+ ; _ : forall A, rel (Class.unit term1) (@Class.unit _ term2 A)
+ ; _ : forall A B C t1 t2, rel t1 t2 -> rel (Class.injl term1 t1) (@Class.injl _ term2 A B C t2)
+ ; _ : forall A B C t1 t2, rel t1 t2 -> rel (Class.injr term1 t1) (@Class.injr _ term2 A B C t2)
+ ; _ : forall A B C D s1 s2 t1 t2, rel s1 s2 -> rel t1 t2 -> rel (Class.case term1 s1 t1) (@Class.case _ term2 A B C D s2 t2)
+ ; _ : forall A B C s1 s2 t1 t2, rel s1 s2 -> rel t1 t2 -> rel (Class.pair term1 s1 t1) (@Class.pair _ term2 A B C s2 t2)
+ ; _ : forall A B C t1 t2, rel t1 t2 -> rel (Class.take term1 t1) (@Class.take _ term2 A B C t2)
+ ; _ : forall A B C t1 t2, rel t1 t2 -> rel (Class.drop term1 t1) (@Class.drop _ term2 A B C t2)
+ }.
+
+Definition Reynolds {A B} (x y : forall (term : type), term A B) : Prop :=
+  forall (term1 term2 : type) (R : ReynoldsRel term1 term2), R A B (x term1) (y term2).
+
+Definition Parametric {A B} (x : forall (term : type), term A B) : Prop := Reynolds x x.
+
+Section Term.
+
+Fixpoint eval {A B} (x : Simplicity.Core.Term A B) {term : type} : term A B :=
+match x in Simplicity.Core.Term A B return term A B with
+| Simplicity.Core.iden => Class.iden term
+| Simplicity.Core.comp s t => Class.comp term (eval s) (eval t)
+| Simplicity.Core.unit => Class.unit term
+| Simplicity.Core.injl t => Class.injl term (eval t)
+| Simplicity.Core.injr t => Class.injr term (eval t)
+| Simplicity.Core.case s t => Class.case term (eval s) (eval t)
+| Simplicity.Core.pair s t => Class.pair term (eval s) (eval t)
+| Simplicity.Core.take t => Class.take term (eval t)
+| Simplicity.Core.drop t => Class.drop term (eval t)
+end.
+
+Lemma eval_Parametric {A B} (x : Simplicity.Core.Term A B) : Parametric (@eval A B x).
+Proof.
+intros term1 term2 [R].
+induction x; simpl; auto.
+Qed.
+
+Canonical Structure Term : type := Pack (Class.Class
   Simplicity.Core.Term
   (@Simplicity.Core.iden)
   (@Simplicity.Core.comp)
@@ -34,19 +74,146 @@ Definition TermAlg : type := Pack (Class.Class
   (@Simplicity.Core.drop)
 ).
 
+Lemma eval_Term {A B} (x : Simplicity.Core.Term A B) : eval x = x.
+Proof.
+induction x; simpl; congruence.
+Qed.
+
+Lemma term_eval {A B} (x : forall (term : type), term A B) (Hx : Parametric x) (term : type) :
+  x term = eval (x Term).
+Proof.
+refine (Hx _ _ (Build_ReynoldsRel Term term (fun a b x y => y = eval x) _ _ _ _ _ _ _ _ _));
+intros; simpl; congruence.
+Qed.
+
+End Term.
+
 End Core.
 
-Coercion Core.alg : Core.type >-> Funclass.
+Coercion Core.rel : Core.ReynoldsRel >-> Funclass.
+Coercion Core.carrier : Core.type >-> Funclass.
 
-Definition iden {term : Core.type} {a : Ty} : term a a := Core.Class.iden (Core.class_of term).
-Definition comp {term : Core.type} {a b c : Ty} : term a b -> term b c -> term a c := Core.Class.comp (Core.class_of term).
-Definition unit {term : Core.type} {a : Ty} : term a Unit := Core.Class.unit (Core.class_of term).
-Definition injl {term : Core.type} {a b c : Ty} : term a b -> term a (Sum b c) := Core.Class.injl (Core.class_of term).
-Definition injr {term : Core.type} {a b c : Ty} : term a c -> term a (Sum b c) := Core.Class.injr (Core.class_of term).
-Definition case {term : Core.type} {a b c d : Ty} : term (Prod a c) d -> term (Prod b c) d -> term (Prod (Sum a b) c) d := Core.Class.case (Core.class_of term).
-Definition pair {term : Core.type} {a b c : Ty} : term a b -> term a c -> term a (Prod b c) := Core.Class.pair (Core.class_of term).
-Definition take {term : Core.type} {a b c : Ty} : term a c -> term (Prod a b) c := Core.Class.take (Core.class_of term).
-Definition drop {term : Core.type} {a b c : Ty} : term b c -> term (Prod a b) c := Core.Class.drop (Core.class_of term).
+Section Core_Combinators.
+
+Definition iden {A} {term : Core.type} : term A A := Core.Class.iden (Core.class_of term).
+Definition comp {A B C} {term : Core.type} : term A B -> term B C -> term A C := Core.Class.comp (Core.class_of term).
+Definition unit {A} {term : Core.type} : term A Unit := Core.Class.unit (Core.class_of term).
+Definition injl {A B C} {term : Core.type} : term A B -> term A (B + C) := Core.Class.injl (Core.class_of term).
+Definition injr {A B C} {term : Core.type} : term A C -> term A (B + C) := Core.Class.injr (Core.class_of term).
+Definition case {A B C D} {term : Core.type} : term (A * C) D -> term (B * C) D -> term ((A + B) * C) D := Core.Class.case (Core.class_of term).
+Definition pair {A B C} {term : Core.type} : term A B -> term A C -> term A (B * C) := Core.Class.pair (Core.class_of term).
+Definition take {A B C} {term : Core.type} : term A C -> term (A * B) C := Core.Class.take (Core.class_of term).
+Definition drop {A B C} {term : Core.type} : term B C -> term (A * B) C := Core.Class.drop (Core.class_of term).
+
+Lemma iden_Parametric {term1 term2 : Core.type} (R : Core.ReynoldsRel term1 term2)
+  {A} : R A A iden iden.
+Proof.
+unfold iden.
+destruct R as [R].
+simpl; auto.
+Qed.
+
+Lemma comp_Parametric {term1 term2 : Core.type} (R : Core.ReynoldsRel term1 term2)
+  {A B C} s1 s2 t1 t2 : R A B s1 s2 -> R B C t1 t2 -> R A C (comp s1 t1) (comp s2 t2).
+Proof.
+unfold comp.
+destruct R as [R].
+simpl; auto.
+Qed.
+
+Lemma unit_Parametric {term1 term2 : Core.type} (R : Core.ReynoldsRel term1 term2)
+  {A} : R A Unit unit unit.
+Proof.
+unfold unit.
+destruct R as [R].
+simpl; auto.
+Qed.
+
+Lemma injl_Parametric {term1 term2 : Core.type} (R : Core.ReynoldsRel term1 term2)
+  {A B C} t1 t2 : R A B t1 t2 -> R A (B + C) (injl t1) (injl t2).
+Proof.
+unfold injl.
+destruct R as [R].
+simpl; auto.
+Qed.
+
+Lemma injr_Parametric {term1 term2 : Core.type} (R : Core.ReynoldsRel term1 term2)
+  {A B C} t1 t2 : R A C t1 t2 -> R A (B + C) (injr t1) (injr t2).
+Proof.
+unfold injr.
+destruct R as [R].
+simpl; auto.
+Qed.
+
+Lemma case_Parametric {term1 term2 : Core.type} (R : Core.ReynoldsRel term1 term2)
+  {A B C D} s1 s2 t1 t2 : R (A * C) D s1 s2 -> R (B * C) D t1 t2 -> R ((A + B) * C) D (case s1 t1) (case s2 t2).
+Proof.
+unfold case.
+destruct R as [R].
+simpl; auto.
+Qed.
+
+Lemma pair_Parametric {term1 term2 : Core.type} (R : Core.ReynoldsRel term1 term2)
+  {A B C} s1 s2 t1 t2 : R A B s1 s2 -> R A C t1 t2 -> R A (B * C) (pair s1 t1) (pair s2 t2).
+Proof.
+unfold pair.
+destruct R as [R].
+simpl; auto.
+Qed.
+
+Lemma take_Parametric {term1 term2 : Core.type} (R : Core.ReynoldsRel term1 term2)
+  {A B C} t1 t2 : R A C t1 t2 -> R (A * B) C (take t1) (take t2).
+Proof.
+unfold take.
+destruct R as [R].
+simpl; auto.
+Qed.
+
+Lemma drop_Parametric {term1 term2 : Core.type} (R : Core.ReynoldsRel term1 term2)
+  {A B C} t1 t2 : R B C t1 t2 -> R (A * B) C (drop t1) (drop t2).
+Proof.
+unfold drop.
+destruct R as [R].
+simpl; auto.
+Qed.
+
+End Core_Combinators.
+
+Create HintDb parametricity.
+Hint Immediate iden_Parametric : parametricity.
+Hint Resolve comp_Parametric : parametricity.
+Hint Immediate unit_Parametric : parametricity.
+Hint Resolve injl_Parametric : parametricity.
+Hint Resolve injr_Parametric : parametricity.
+Hint Resolve case_Parametric : parametricity.
+Hint Resolve pair_Parametric : parametricity.
+Hint Resolve take_Parametric : parametricity.
+Hint Resolve drop_Parametric : parametricity.
 
 Notation "s &&& t" := (pair s t) (at level 70, right associativity) : term_scope.
 Notation "s >>> t" := (comp s t) (at level 90, right associativity) : term_scope.
+
+Section CoreSem.
+
+Definition CoreSem : Core.type := Core.Pack (Core.Class.Class (fun A B => A -> B)
+  (fun A a => a)
+  (fun A B C s t a => t (s a))
+  (fun A _ => tt)
+  (fun A B C t a => inl (t a))
+  (fun A B C t a => inr (t a))
+  (fun A B C D s t p => let (ab, c) := p in
+    match ab with
+    | inl a => s (a, c)
+    | inr b => t (b, c)
+    end)
+  (fun A B C s t a => (s a, t a))
+  (fun A B C t ab => t (fst ab))
+  (fun A B C t ab => t (snd ab))
+).
+
+Lemma CoreSem_correct {A B} (x : Simplicity.Core.Term A B) : Simplicity.Core.eval x = Core.eval x (term := CoreSem).
+Proof.
+induction x; simpl; try first [rewrite IHx | rewrite IHx1, IHx2]; reflexivity.
+Qed.
+
+End CoreSem.
