Coq/Simplicity/Arith.v
@@ -2,11 +2,175 @@ Require Import Simplicity.Ty.
 Require Import Simplicity.Alg.
 Require Import Simplicity.Bit.
 
+Local Open Scope ty_scope.
+Local Open Scope term_scope.
+
 Fixpoint Word (n : nat) :=
 match n with
 | O => Bit
-| (S n) => let rec := Word n in Prod rec rec
+| S n => let rec := Word n in Prod rec rec
 end.
 
-Definition adderBit {term : Core.type} : term (Prod Bit Bit) (Prod Bit Bit) :=
+Section Definitions.
+
+Definition adderBit {term : Core.type} : term (Bit * Bit) (Bit * Bit) :=
   cond (iden &&& not iden) (false &&& iden).
+
+Definition fullAdderBit {term : Core.type} : term ((Bit * Bit) * Bit) (Bit * Bit) :=
+  let add := adderBit in
+    take add &&& drop iden
+>>> take (take iden) &&& (take (drop iden) &&& drop iden >>> add)
+>>> cond true (take iden) &&& drop (drop iden).
+
+Definition buildFullAdder {W} {term : Core.type} (rec : term ((W * W) * Bit) (Bit * W)) :
+  term (((W * W) * (W * W)) * Bit) (Bit * (W * W)) :=
+    take (take (take iden) &&& drop (take iden))
+&&& (take (take (drop iden) &&& drop (drop iden)) &&& drop iden >>> rec)
+>>> (take iden &&& drop (take iden) >>> rec) &&& drop (drop iden)
+>>> take (take iden) &&& (take (drop iden) &&& drop iden).
+
+Fixpoint fullAdder {n : nat} {term : Core.type} : term ((Word n * Word n) * Bit) (Bit * Word n) :=
+match n with
+| O => fullAdderBit
+| S n => buildFullAdder fullAdder
+end.
+
+Definition buildAdder {W} {term : Core.type} (fa : term ((W * W) * Bit) (Bit * W)) (rec : term (W * W) (Bit * W)) :
+  term ((W * W) * (W * W)) (Bit * (W * W)) :=
+    (take (take iden) &&& drop (take iden))
+&&& (take (drop iden) &&& drop (drop iden) >>> rec)
+>>> (take iden &&& drop (take iden) >>> fa) &&& drop (drop iden)
+>>> take (take iden) &&& (take (drop iden) &&& drop iden).
+
+Fixpoint adder {n : nat} {term : Core.type} : term (Word n * Word n) (Bit * Word n) :=
+match n with
+| O => adderBit
+| S n => buildAdder fullAdder adder
+end.
+
+Definition fullMultiplierBit {term : Core.type} : term ((Bit * Bit) * (Bit * Bit)) (Bit * Bit) :=
+    drop iden &&& take (cond iden false)
+>>> fullAdderBit.
+
+Definition buildFullMultiplier {W} {term : Core.type} (rec : term ((W * W) * (W * W)) (W * W)) :
+  term (((W * W) * (W * W)) * ((W * W) * (W * W))) (((W * W) * (W * W))) :=
+    take ((take (take iden) &&& drop (take iden)) &&& take (drop iden))
+&&& ((take (take (take iden) &&& drop (drop iden)) &&& drop (take (take iden) &&& drop (take iden)) >>> rec)
+&&& (take (take (drop iden) &&& drop (drop iden)) &&& drop (take (drop iden) &&& drop (drop iden)) >>> rec))
+>>> (take (take iden) &&& (take (take (drop iden) &&& drop iden) &&& drop (take (drop iden) &&& drop (take iden)) >>> rec))
+&&& (drop (take (take iden) &&& drop (drop iden)))
+>>> (take (take iden) &&& (take (drop (take iden)) &&& drop (take iden)) >>> rec) &&& (take (drop (drop iden)) &&& drop (drop iden)).
+
+Fixpoint fullMultiplier {n : nat} {term : Core.type} : term ((Word n * Word n) * (Word n * Word n)) (Word n * Word n) :=
+match n with
+| O => fullMultiplierBit
+| S n => buildFullMultiplier fullMultiplier
+end.
+
+Definition multiplierBit {term : Core.type} : term (Bit * Bit) (Bit * Bit) :=
+    false &&& cond iden false.
+
+Definition buildMultiplier {W} {term : Core.type} (fmul : term ((W * W) * (W * W)) (W * W)) (rec : term (W * W) (W * W)) :
+  term ((W * W) * (W * W)) ((W * W) * (W * W)) :=
+    ((take (take iden) &&& drop (take iden)) &&& take (drop iden))
+&&& ((take (take iden) &&& drop (drop iden) >>> rec)
+&&& (take (drop iden) &&& drop (drop iden) >>> rec))
+>>> (take (take iden) &&& (take (take (drop iden) &&& drop iden) &&& drop (take (drop iden) &&& drop (take iden)) >>> fmul))
+&&& (drop (take (take iden) &&& drop (drop iden)))
+>>> (take (take iden) &&& (take (drop (take iden)) &&& drop (take iden)) >>> fmul) &&& (take (drop (drop iden)) &&& drop (drop iden)).
+
+Fixpoint multiplier {n : nat} {term : Core.type} : term (Word n * Word n) (Word n * Word n) :=
+match n with
+| O => multiplierBit
+| S n => buildMultiplier fullMultiplier multiplier
+end.
+
+End Definitions.
+
+Lemma adderBit_Parametric {term1 term2 : Core.type} (R : Core.ReynoldsRel term1 term2) : R _ _ adderBit adderBit.
+Proof.
+unfold adderBit.
+auto with parametricity.
+Qed.
+Hint Resolve adderBit_Parametric : parametricity.
+
+Lemma fullAdderBit_Parametric {term1 term2 : Core.type} (R : Core.ReynoldsRel term1 term2) : R _ _ fullAdderBit fullAdderBit.
+Proof.
+unfold fullAdderBit.
+auto 10 with parametricity.
+Qed.
+Hint Resolve fullAdderBit_Parametric : parametricity.
+
+Lemma buildFullAdder_Parametric {term1 term2 : Core.type} (R : Core.ReynoldsRel term1 term2)
+  {W} t1 t2 : R _ (Bit * W) t1 t2 -> R _ _ (buildFullAdder t1) (buildFullAdder t2).
+Proof.
+unfold buildFullAdder.
+auto 10 with parametricity.
+Qed.
+Hint Resolve buildFullAdder_Parametric : parametricity.
+
+Lemma fullAdder_Parametric {term1 term2 : Core.type} (R : Core.ReynoldsRel term1 term2)
+  {n} : R _ _ fullAdder (@fullAdder n _).
+Proof.
+induction n; simpl; auto with parametricity.
+Qed.
+Hint Resolve fullAdder_Parametric : parametricity.
+
+Lemma buildAdder_Parametric {term1 term2 : Core.type} (R : Core.ReynoldsRel term1 term2)
+  {W} s1 s2 t1 t2 : R _ (Bit * W) s1 s2 -> R _ (Bit * W) t1 t2 -> R _ _ (buildAdder s1 t1) (buildAdder s2 t2).
+Proof.
+unfold buildAdder.
+auto 10 with parametricity.
+Qed.
+Hint Resolve buildAdder_Parametric : parametricity.
+
+Lemma adder_Parametric {term1 term2 : Core.type} (R : Core.ReynoldsRel term1 term2)
+  {n} : R _ _ adder (@adder n _).
+Proof.
+induction n; simpl; auto with parametricity.
+Qed.
+Hint Resolve adder_Parametric : parametricity.
+
+Lemma fullMultiplierBit_Parametric {term1 term2 : Core.type} (R : Core.ReynoldsRel term1 term2) : R _ _ fullMultiplierBit fullMultiplierBit.
+Proof.
+unfold fullMultiplierBit.
+auto with parametricity.
+Qed.
+Hint Resolve fullMultiplierBit_Parametric : parametricity.
+
+Lemma buildFullMultiplier_Parametric {term1 term2 : Core.type} (R : Core.ReynoldsRel term1 term2)
+  {W} t1 t2 : R _ (W * W) t1 t2 -> R _ _ (buildFullMultiplier t1) (buildFullMultiplier t2).
+Proof.
+unfold buildFullMultiplier.
+auto 15 with parametricity.
+Qed.
+Hint Resolve buildFullMultiplier_Parametric : parametricity.
+
+Lemma fullMultiplier_Parametric {term1 term2 : Core.type} (R : Core.ReynoldsRel term1 term2)
+  {n} : R _ _ fullMultiplier (@fullMultiplier n _).
+Proof.
+induction n; simpl; auto with parametricity.
+Qed.
+Hint Resolve fullMultiplier_Parametric : parametricity.
+
+Lemma multiplierBit_Parametric {term1 term2 : Core.type} (R : Core.ReynoldsRel term1 term2) : R _ _ multiplierBit multiplierBit.
+Proof.
+unfold multiplierBit.
+auto with parametricity.
+Qed.
+Hint Resolve multiplierBit_Parametric : parametricity.
+
+Lemma buildMultiplier_Parametric {term1 term2 : Core.type} (R : Core.ReynoldsRel term1 term2)
+  {W} s1 s2 t1 t2 : R _ (W * W) s1 s2 -> R _ (W * W) t1 t2 -> R _ _ (buildMultiplier s1 t1) (buildMultiplier s2 t2).
+Proof.
+unfold buildMultiplier.
+auto 15 with parametricity.
+Qed.
+Hint Resolve buildMultiplier_Parametric : parametricity.
+
+Lemma multiplier_Parametric {term1 term2 : Core.type} (R : Core.ReynoldsRel term1 term2)
+  {n} : R _ _ multiplier (@multiplier n _).
+Proof.
+induction n; simpl; auto with parametricity.
+Qed.
+Hint Resolve multiplier_Parametric : parametricity.
