Coq/Simplicity/Bit.v
@@ -1,15 +1,52 @@
 Require Import Simplicity.Ty.
 Require Import Simplicity.Alg.
 
-Open Scope term_scope.
+Local Open Scope ty_scope.
+Local Open Scope term_scope.
 
-Definition Bit := Sum Unit Unit.
+Notation Bit := (Unit + Unit).
 
-Definition false {term : Core.type} {a : Ty} : term a Bit := injl unit.
-Definition true {term : Core.type} {a : Ty} : term a Bit := injr unit.
+Section Definitions.
 
-Definition cond {term : Core.type} {a b : Ty} (thn els : term a b) : term (Prod Bit a) b :=
+Definition false {A} {term : Core.type} : term A Bit := injl unit.
+Definition true {A} {term : Core.type} : term A Bit := injr unit.
+
+Definition cond {A B} {term : Core.type} (thn els : term A B) : term (Bit * A) B :=
   case (drop els) (drop thn).
 
-Definition not {term : Core.type} {a : Ty} (t : term a Bit) : term a Bit :=
+Definition not {A} {term : Core.type} (t : term A Bit) : term A Bit :=
   t &&& unit >>> cond false true.
+
+End Definitions.
+
+Lemma false_Parametric {term1 term2 : Core.type} (R : Core.ReynoldsRel term1 term2)
+  {A} : R A Bit false false.
+Proof.
+unfold false.
+auto with parametricity.
+Qed.
+Hint Immediate false_Parametric : parametricity.
+
+Lemma true_Parametric {term1 term2 : Core.type} (R : Core.ReynoldsRel term1 term2)
+  {A} : R A Bit true true.
+Proof.
+unfold true.
+auto with parametricity.
+Qed.
+Hint Immediate true_Parametric : parametricity.
+
+Lemma cond_Parametric {term1 term2 : Core.type} (R : Core.ReynoldsRel term1 term2)
+  {A B} s1 s2 t1 t2 : R A B s1 s2 -> R A B t1 t2 -> R (Bit * A) B (cond s1 t1) (cond s2 t2).
+Proof.
+unfold cond.
+auto with parametricity.
+Qed.
+Hint Resolve cond_Parametric : parametricity.
+
+Lemma not_Parametric {term1 term2 : Core.type} (R : Core.ReynoldsRel term1 term2)
+  {A} t1 t2 : R A Bit t1 t2 -> R A Bit (not t1) (not t2).
+Proof.
+unfold not.
+auto with parametricity.
+Qed.
+Hint Resolve not_Parametric : parametricity.
