Coq/Simplicity/Core.v
@@ -1,18 +1,18 @@
 Require Import Simplicity.Ty.
 
 Inductive Term : Ty -> Ty -> Set :=
-| iden : forall {A : Ty}, Term A A
-| comp : forall {A B C : Ty}, Term A B -> Term B C -> Term A C
-| unit : forall {A : Ty}, Term A Unit
-| injl : forall {A B C : Ty}, Term A B -> Term A (Sum B C)
-| injr : forall {A B C : Ty}, Term A C -> Term A (Sum B C)
-| case : forall {A B C D : Ty},
+| iden : forall {A}, Term A A
+| comp : forall {A B C}, Term A B -> Term B C -> Term A C
+| unit : forall {A}, Term A Unit
+| injl : forall {A B C}, Term A B -> Term A (Sum B C)
+| injr : forall {A B C}, Term A C -> Term A (Sum B C)
+| case : forall {A B C D},
     Term (Prod A C) D -> Term (Prod B C) D -> Term (Prod (Sum A B) C) D
-| pair : forall {A B C : Ty}, Term A B -> Term A C -> Term A (Prod B C)
-| take : forall {A B C : Ty}, Term A C -> Term (Prod A B) C
-| drop : forall {A B C : Ty}, Term B C -> Term (Prod A B) C.
+| pair : forall {A B C}, Term A B -> Term A C -> Term A (Prod B C)
+| take : forall {A B C}, Term A C -> Term (Prod A B) C
+| drop : forall {A B C}, Term B C -> Term (Prod A B) C.
 
-Fixpoint eval {A B : Ty} (x : Term A B) : tySem A -> tySem B :=
+Fixpoint eval {A B} (x : Term A B) : tySem A -> tySem B :=
 match x in Term A B return tySem A -> tySem B with
 | iden => fun a => a
 | comp s t => fun a => eval t (eval s a)
