Coq/Simplicity/Ty.v
@@ -2,6 +2,7 @@ Inductive Ty : Set :=
 | Unit : Ty
 | Sum  : Ty -> Ty -> Ty
 | Prod : Ty -> Ty -> Ty.
+Bind Scope ty_scope with Ty.
 
 Fixpoint tySem (X : Ty) : Set :=
 match X with
@@ -9,3 +10,7 @@ match X with
 | Sum A B => tySem A + tySem B
 | Prod A B => tySem A * tySem B
 end.
+
+Notation "A + B" := (Sum A B) : ty_scope.
+Notation "A * B" := (Prod A B) : ty_scope.
+Coercion tySem : Ty >-> Sortclass.
